theories/Padded.v
@@ -77,3 +77,59 @@ Proof.
     + constructor. right. eauto.
     + constructor. right. eauto.
 Qed.
+
+Global Instance pad_Proper {b1 b2 E R} : Proper (eqit eq b1 b2 ==> eqit eq b1 b2) (@pad E R).
+Proof.
+  pcofix CIH.
+  intros t1 t2 Ht12. pstep. red. unfold pad.
+  punfold Ht12. red in Ht12. hinduction Ht12 before r;
+    intros; cbn; eauto.
+  - constructor. auto.
+  - constructor. pclearbot. right. eapply CIH; eauto.
+  - constructor. left. pstep. constructor. pclearbot. right.
+    eapply CIH; eauto. apply REL.
+  - constructor; auto.
+  - constructor; auto.
+Qed.
+
+Theorem pad_ret E R (r : R) : @eq_itree E R R eq (pad (Ret r)) (Ret r).
+Proof. unfold pad. cbn. pstep. red. cbn. constructor. auto. Qed.
+
+Theorem pad_tau E R : forall (t : itree E R), pad (Tau t) ≅ Tau (pad t).
+Proof.
+  intros. pstep. red. cbn. constructor. left.
+  enough (pad t ≅ pad t). auto. reflexivity.
+Qed.
+
+Theorem pad_vis E R A e (k : A -> itree E R) : 
+  pad (Vis e k) ≅ Vis e (fun a => Tau (pad (k a))).
+Proof.
+  intros. pstep. red. cbn. constructor. left.
+  enough (Tau (pad (k v)) ≅ Tau (pad (k v)) ). auto. reflexivity.
+Qed.
+ 
+Theorem pad_bind E R S (k : R -> itree E S) : 
+  forall t, pad (ITree.bind t k) ≅ ITree.bind (pad t) (fun r => pad (k r)).
+Proof.
+  ginit. gcofix CIH. intros. destruct (observe t) eqn : Heq; symmetry in Heq; apply simpobs in Heq;
+    rewrite Heq.
+  - rewrite pad_ret. setoid_rewrite bind_ret_l. gfinal.
+    right. eapply paco2_mon with (r := bot2); intros; try contradiction.
+    enough (pad (k r0) ≅ pad (k r0)); auto. reflexivity.
+  - rewrite bind_tau. repeat rewrite pad_tau. rewrite bind_tau.
+    gstep. constructor. gfinal. left. eapply CIH.
+  - rewrite bind_vis. repeat rewrite pad_vis. rewrite bind_vis.
+    setoid_rewrite bind_tau. gstep. constructor.
+    gstep. constructor. gfinal. left. eauto.
+Qed.
+
+Theorem pad_iter E R S (body : R -> itree E (R + S)):
+  forall r, pad (ITree.iter body r) ≅ ITree.iter (fun r => pad (body r)) r.
+Proof.
+  ginit. gcofix CIH.
+  intros. setoid_rewrite unfold_iter. rewrite pad_bind.
+  guclo eqit_clo_bind. econstructor.
+  reflexivity. intros. subst. destruct u2.
+  - rewrite pad_tau. gstep. constructor. gfinal. left. eauto.
+  - rewrite pad_ret. gstep. constructor. auto.
+Qed.
