theories/RefinementEutt.v
@@ -1,0 +1,46 @@
+From Coq Require Export Morphisms Setoid Program.Equality.
+From ITree Require Export ITree ITreeFacts Eq.Rutt.
+From Paco Require Import paco.
+From Coq Require Export Eqdep EqdepFacts.
+
+Require Export HeterogeneousEventRelations Padded Refinement.
+
+Variant EvEq {E : Type -> Type} : forall (A B : Type), E A -> E B -> Prop :=
+  | eveq (A : Type) (e : E A) : EvEq A A e e.
+
+Variant EvEqAns {E : Type -> Type} : forall A B, E A -> E B -> A -> B -> Prop :=
+  | eveqans A (e : E A) (a : A) : EvEqAns A A e e a a.
+
+
+Lemma eutt_to_refines E R : forall (t1 t2 : itree_spec E R),
+    padded t1 -> padded t2 ->
+    t1 ≈ t2 -> refines EvEq EvEqAns eq t1 t2.
+Proof.
+  pcofix CIH. intros.
+  pstep. red. punfold H2. red in H2. punfold H0. red in H0.
+  punfold H1. red in H1.
+  hinduction H2 before r; intros; try destruct e; pclearbot; eauto.
+  - constructor. right. eapply CIH; eauto.
+    inv H0. pclearbot. auto. inv H1. pclearbot. auto.
+  - constructor. constructor. intros. inv H. inj_existT. subst.
+    inv H0. inv H1. inj_existT. subst. right. eapply CIH; eauto.
+    pstep. constructor. auto. pstep. constructor. auto.
+    apply REL.
+  - inv H0. inv H1. inj_existT. subst. constructor.
+    intros. eapply refines_forallL. constructor. right. eapply CIH; pclearbot; eauto.
+    eapply H2. eapply H0. setoid_rewrite <- tau_eutt. eapply REL.
+  - inv H0. inv H1. inj_existT. subst. constructor. intros.
+    eapply  refines_existsR. constructor. right. pclearbot. eapply CIH; eauto.
+    apply H2. apply H0. setoid_rewrite <- tau_eutt. apply REL.
+  - constructor. inv H0. pclearbot. punfold H3.
+  - constructor. inv H1. pclearbot. punfold H3.
+Qed.
+
+Lemma refines_eutt_padded_r E1 E2 R1 R2 RE REAns RR : 
+  forall (t1 : itree_spec E1 R1) (t2 t3 : itree_spec E2 R2),
+    padded t1 -> padded t2 -> padded t3 -> t2 ≈ t3 ->
+    refines RE REAns RR t1 t2 -> refines RE REAns RR t1 t3.
+Proof.
+  intros. apply eutt_to_refines in H2; auto.
+  (* this approach would only work if *)
+Abort.
